src/Prog.v
@@ -1,159 +1,254 @@
 From Stdlib Require Import Lists.List. Import ListNotations.
 From Stdlib Require Import Strings.String.
 From stdpp Require Import base gmap.
-From MRC Require Import Options.
+From MRC Require Import Prelude.
+From MRC Require Import SeqNotation.
 From MRC Require Import Tactics.
 From MRC Require Import Model.
 From MRC Require Import Stdppp.
 From MRC Require Import PredCalc.
 
+Open Scope stdpp_scope.
+
 Section prog.
   Context {M : model}.
   Local Notation term := (term (value M)).
+  Local Notation final_term := (final_term (value M)).
   Local Notation formula := (formula (value M)).
   Local Notation final_formula := (final_formula (value M)).
 
+  Variant asgn_rhs_term :=
+    | OpenRhsTerm
+    | FinalRhsTerm (t : final_term).
+
   Inductive prog : Type :=
-  | PAsgn (x : final_variable) (t : term)
+  | PAsgn (asgns : list (final_variable * asgn_rhs_term))
   | PSeq (p1 p2 : prog)
   | PIf (gcmds : list (formula * prog))
-  (* | PWhile (g : formula) (p: prog) (inv : formula) (variant : variable) *)
   | PSpec (w : list final_variable) (pre : final_formula) (post : formula)
   | PVar (x : variable) (p : prog)
   | PConst (x : variable) (p : prog).
 
-  Axiom re : (prog → prog) → prog.
+  Notation asgn_list := (list (final_variable * asgn_rhs_term)).
+  Notation gcmd_list := (list (formula * prog)).
+  Definition gcmd_comprehension (gs : list formula) (f : formula → prog) : gcmd_list :=
+    map (λ A, (A, f A)) gs.
 
   Fixpoint modified_final_vars p : list final_variable :=
     match p with
-    | PAsgn x t => [x]
+    | PAsgn asgns => fst <$> asgns
     | PSeq p1 p2 => modified_final_vars p1 ++ modified_final_vars p2
     | PIf gcmds => mjoin ((modified_final_vars ∘ snd) <$> gcmds)
-    (* | PWhile _ p _ _ => modified_ni_vars p *)
     | PSpec w pre post => w
     | PVar x p => modified_final_vars p
     | PConst x p => modified_final_vars p
     end.
 
-  Definition modified_vars p : list variable := final_var_var <$> modified_final_vars p.
+  Definition modified_vars p : list variable := as_var_F (modified_final_vars p).
   Notation "'Δ' p" := (modified_vars p) (at level 50).
 
   Fixpoint prog_fvars p : gset variable :=
     match p with
-    | PAsgn x t => {[final_var_var x]}
+    | PAsgn asgns => list_to_set (as_var_F (fst <$> asgns))
     | PSeq p1 p2 => prog_fvars p1 ∪ prog_fvars p2
     | PIf gcmds => ⋃ ((prog_fvars ∘ snd) <$> gcmds)
-    (* | PWhile _ p _ _ => prog_fvars p *)
-    | PSpec w pre post => list_to_set (final_var_var <$> w) ∪ formula_fvars pre ∪ formula_fvars post
+    | PSpec w pre post => list_to_set (as_var_F w) ∪ formula_fvars pre ∪ formula_fvars post
     | PVar x p => prog_fvars p ∖ {[x]}
     | PConst x p => prog_fvars p ∖ {[x]}
   end.
 
-  Fixpoint any_guard (gcmds : list (formula * prog)) : formula :=
+  Fixpoint any_guard (gcmds : gcmd_list) : formula :=
     match gcmds with
     | [] => <! true !>
-    | (g, _)::cmds => <! g ∨ `any_guard cmds` !>
+    | (g, _)::cmds => <! g ∨ $(any_guard cmds) !>
     end.
 
-  Fixpoint all_cmds (gcmds : list (formula * prog)) (A : formula) : formula :=
+  Fixpoint all_cmds (gcmds : gcmd_list) (A : formula) : formula :=
     match gcmds with
     | [] => <! true !>
-    | (g, _)::cmds => <! (g => A) ∧ `all_cmds cmds A` !>
+    | (g, _)::cmds => <! (g ⇔ A) ∧ $(all_cmds cmds A) !>
     end.
 
-  Fixpoint spec_post_wp (w : list ni_variable) post A : formula :=
-    match w with
-    | [] => <! post => A !>
-    | h :: t => <! forall h, `spec_post_wp t post A` !>
-    end.
-
-  Fixpoint subst_initials A (w : list ni_variable) : formula :=
+  Fixpoint subst_initials A (w : list final_variable) : formula :=
     match w with
     | [] => A
-    | x :: xs => subst_initials (A[(x)₀ \ x]) xs
+    | x :: xs => subst_initials (A[₀x \ x]) xs
     end.
+
+  Fixpoint split_asgn_list (asgns : asgn_list)
+      : (list final_variable * list (final_variable * final_term)) :=
+    match asgns with
+      | [] => ([], [])
+      | (x, OpenRhsTerm)::rest =>
+          let (opens, asgns) := split_asgn_list rest in
+          (x :: opens, asgns)
+      | (x, FinalRhsTerm t)::rest =>
+          let (opens, asgns) := split_asgn_list rest in
+          (opens, (x, t)::asgns)
+    end.
+
 
   Fixpoint wp (p : prog) (A : formula) : formula :=
     match p with
-    | PAsgn x e => A[x \ e]
+    | PAsgn asgns => A[x \ e]
     | PSeq p1 p2 => wp p1 (wp p2 A)
-    | PIf gcs => <! `any_guard (gcs)` ∧ `all_cmds (gcs) A` !>
-    | PWhile g p inv v =>
-        let x := fresh_var (raw_var "x") (formula_fvars inv ∪ prog_fvars p ∪ formula_fvars A) in
-        <! forall* Δ p`,
-            (inv ∧ g => `wp p inv`) ∧
-            (inv ∧ ¬ g => A) ∧
-            (inv ∧ g ∧ v = x => `wp p (<! v < x !>)`) !>
-    | PSpec w pre post => <! pre ∧ `subst_initials (spec_post_wp w post A) w` !>
-    | PVar x p => <! forall x, `wp p A` !>
-    | PConst x p => <! exists x, `wp p A` !>
+    | PIf gcs => <! $(any_guard gcs) ∧ $(all_cmds gcs A) !>
+    | PSpec w pre post => <! pre ∧ $(subst_initials (<! ∀* $(as_var_F w), post ⇒ A !>) w) !>
+    | PVar x p => <! ∀ x, $(wp p A) !>
+    | PConst x p => <! ∃ x, $(wp p A) !>
     end.
 
-  Definition refines (p1 p2 : prog) :=
-    ∀ A : ni_formula,
+  (* ******************************************************************* *)
+  (* definition and properties of ⊑ and ≡ on progs                       *)
+  (* ******************************************************************* *)
+  Global Instance refines : SqSubsetEq prog := λ p1 p2,
+    ∀ A : final_formula,
       (∀ x, x ∈ formula_fvars A → var_is_initial x = false) ->
       wp p1 A ⇛ (wp p2 A).
 
-  Notation "x '⊑' y" := (refines x y)
-                          (in custom prog at level 60,
-                              x custom prog,
-                              y custom prog at level 95).
+  Global Instance pequiv : Equiv prog := λ p1 p2, p1 ⊑ p2 ∧ p2 ⊑ p1.
+  Global Instance refines_refl : Reflexive refines.
+  Proof with auto. intros ? ? ?. reflexivity. Qed.
+
+  Global Instance refines_trans : Transitive refines.
+  Proof with auto. intros ? ? ? ? ? ? ?... transitivity (wp y A); naive_solver. Qed.
+
+  Global Instance pequiv_refl : Reflexive pequiv.
+  Proof with auto. split; reflexivity. Qed.
+
+  Global Instance pequiv_sym : Symmetric pequiv.
+  Proof with auto. intros p1 p2. unfold pequiv. naive_solver. Qed.
+
+  Global Instance pequiv_trans : Transitive pequiv.
+  Proof with auto.
+    intros p1 p2 p3 [H12 H21] [H23 H32]. split.
+    - transitivity p2...
+    - transitivity p2...
+  Qed.
+
+  Global Instance pequiv_equiv : Equivalence pequiv.
+  Proof.
+    split.
+    - exact pequiv_refl.
+    - exact pequiv_sym.
+    - exact pequiv_trans.
+  Qed.
+
+  Global Instance refines_antisym : Antisymmetric prog pequiv refines.
+  Proof. intros p1 p2 H12 H21. split; assumption. Qed.
+
+  (* ******************************************************************* *)
+  (* axiomatization of recursive blocks and definition of while          *)
+  (* ******************************************************************* *)
+  Axiom PRec : (prog → prog) → prog.
+
+  Axiom p_rec_unfold_l : ∀ F, PRec F ⊑ F (PRec F).
+  Axiom p_rec_unfold_r : ∀ F, F (PRec F) ⊑ PRec F.
+
+  Lemma p_rec_fixpoint : ∀ F, F (PRec F) ≡ PRec F.
+  Proof.
+    intros. split.
+    - apply p_rec_unfold_r.
+    - apply p_rec_unfold_l.
+  Qed.
+
+  Axiom rec_ind : ∀ F P, F P ≡ P → PRec F ⊑ P.
+
+  (* while g => p    =    re P ⦁ if g then p; P fi er *)
+  Definition PWhile (gcmds : gcmd_list) :=
+    PRec (λ P, PIf gcmds).
+
+
+  (* ******************************************************************* *)
+  (* some extreme programs                                               *)
+  (* ******************************************************************* *)
+  (* Definition abort := PSpec ([]) <! true !> <! false !>. *)
 
 End prog.
 
 Declare Custom Entry prog.
 Declare Custom Entry gcmd.
-Declare Scope prog_scope.
-Declare Custom Entry prog_aux.
-Bind Scope prog_scope with prog.
-Delimit Scope prog_scope with prog.
 
-Notation "<{ e }>" := e (e custom prog_aux) : prog_scope.
-Notation "e" := e (in custom prog_aux at level 0, e custom prog) : prog_scope.
+Notation "<{ e }>" := e (e custom prog) : refiney_scope.
 
-Notation "( x )" := x (in custom prog, x at level 99) : prog_scope.
-Notation "'`' x '`'" := (x)
-                          (in custom prog at level 0, only parsing,
-                              x constr at level 0) : prog_scope.
-Notation "x" := x (in custom prog at level 0, x constr at level 0) : prog_scope.
+Notation "$ e" := e (in custom prog at level 0, e constr at level 0)
+    : refiney_scope.
 
-Notation "x := e" := (PAsgn x e)
-                       (in custom prog at level 95,  x constr at level 0,
-                           e custom formula at level 85, no associativity) : prog_scope.
+Notation "$( e )" := e (in custom prog at level 0, only parsing,
+                           e constr at level 200)
+    : refiney_scope.
 
-Notation "x ; y" := (PSeq x y)
-                      (in custom prog at level 95, right associativity) : prog_scope.
+Notation "x := t" := (PAsgn x t)
+                       (in custom prog at level 95,
+                           x constr at level 0,
+                           t custom term at level 85, no associativity)
+    : refiney_scope.
 
-Notation "x -> y" := ((x, y))
-                       (in custom gcmd at level 60, x custom formula,
-                           y custom prog,
-                           no associativity) : prog_scope.
+Notation "p ; q" := (PSeq p q)
+                      (in custom prog at level 120, right associativity)
+    : refiney_scope.
 
-Notation "'if' | x | .. | y 'fi'" :=
+Notation "A → p" := ((A, p)) (in custom gcmd at level 60,
+                           A custom formula,
+                           p custom prog,
+                           no associativity) : refiney_scope.
+
+Notation "'if' x | .. | y 'fi'" :=
   (PIf (cons (x) .. (cons (y) nil) ..))
     (in custom prog at level 95,
         x custom gcmd,
-        y custom gcmd, no associativity) : prog_scope.
+        y custom gcmd, no associativity) : refiney_scope.
 
-Notation "'while' g 'do' p 'invariant' i 'variant' v 'end'" :=
-  (PWhile g p i v)
+Notation "'if' | g : gs → p 'fi'" := (PIf (gcmd_comprehension gs (λ g, p)))
+                                     (in custom prog at level 95, g name,
+                                         gs global, p custom prog)
+    : refiney_scope.
+
+Notation "'re' p ⦁ F 'er'" := (PRec (λ p, F))
+                                (in custom prog at level 95,
+                                    p name, F custom prog)
+    : refiney_scope.
+
+Notation "'while' A ⟶ p 'end" :=
+  (PWhile A p)
     (in custom prog at level 95,
-        g custom formula, p custom prog, i custom formula, no associativity) : prog_scope.
-
-Notation "x , .. , y : [ p , q ]" :=
-  (PSpec (cons x .. (cons y nil) ..) p q)
+        A custom formula, p custom prog, no associativity) : refiney_scope.
+(* Notation "⟨ x , .. , y ⟩ : [ p , q ]" := *)
+(*   (PSpec (cons x .. (cons y nil) ..) p q) *)
+(*     (in custom prog at level 130, no associativity, *)
+(*         x constr at level 0, y constr at level 0, *)
+(*         p custom formula at level 85, q custom formula at level 85)
+: refiney_scope. *)
+Notation "w : [ p , q ]" :=
+  (PSpec w p q)
     (in custom prog at level 95, no associativity,
-        x constr at level 0, y constr at level 0,
-        p custom formula at level 85, q custom formula at level 85) : prog_scope.
+        w custom seq_notation at level 94,
+        p custom formula at level 85, q custom formula at level 85)
+    : refiney_scope.
 
-Notation "'|[' 'var' x ',' y ']|' " :=
+(* Notation ": [ p , q ]" := *)
+(*   (PSpec ([]) p q) *)
+(*     (in custom prog at level 95, no associativity, *)
+(*         p custom formula at level 85, q custom formula at level 85)
+: refiney_scope. *)
+
+Axiom M : model.
+Axiom p1 p2 : @prog M.
+Axiom pre : @final_formula (value M).
+Axiom post : @formula (value M).
+Axiom x y : final_variable.
+Axiom xs ys : list final_variable.
+Definition pp := <{ $p1 ; $p2 }>.
+Definition pp2 := <{ ∅ : [<! pre !>, post] }>.
+Definition pp3 := <{ x := x }>.
+Print pp2.
+
+Notation "'|[' 'var' x '⦁' y ']|' " :=
   (PVar x y)
     (in custom prog at level 95, no associativity,
-        x constr at level 0, y custom prog) : prog_scope.
+        x constr at level 0, y custom prog) : refiney_scope.
 
-Notation "'|[' 'const' x ',' y ']|' " :=
+Notation "'|[' 'con' x '⦁' y ']|' " :=
   (PConst x y)
     (in custom prog at level 95, no associativity,
-        x constr at level 0, y custom prog at next level) : prog_scope.
-
-Open Scope prog_scope.
+        x constr at level 0, y custom prog at next level) : refiney_scope.
