src/Refinement.v
@@ -1,7 +1,7 @@
 From Stdlib Require Import Lists.List. Import ListNotations.
 From Equations Require Import Equations.
 From stdpp Require Import base tactics listset.
-From MRC Require Import Options.
+From MRC Require Import Prelude.
 From MRC Require Import Tactics.
 From MRC Require Import Model.
 From MRC Require Import Stdppp.
@@ -12,25 +12,15 @@ Section refinement.
   Context {M : model}.
   Local Notation prog := (@prog M).
   Local Notation formula := (formula (value M)).
-  Local Notation ni_formula := (@ni_formula M).
+  Local Notation final_term := (final_term (value M)).
 
   Implicit Types A B C : formula.
-  Implicit Types pre : ni_formula.
+  Implicit Types pre : @final_formula (value M).
   (* Implicit Types w : list variable. *)
-
-  Definition refines (p1 p2 : prog) :=
-    ∀ A : ni_formula,
-      (∀ x, x ∈ formula_fvars A → var_is_initial x = false) ->
-      wp p1 A ⇛ (wp p2 A).
-
-  Notation "x '⊑' y" := (refines x y)
-                          (in custom prog at level 60,
-                              x custom prog,
-                              y custom prog at level 95).
 
   Lemma r_strengthen_post pre post post' w :
     post' ⇛ post ->
-    <{ w : [pre, post] ⊑ w : [pre, post'] }>.
+    <{ w : [pre, post] }> ⊑ <{ w : [pre, post'] }>.
   Proof.
     intros Hent A Hinit. simpl. f_simpl. apply f_forall_ent. intros.
     f_simpl. assumption.
@@ -38,39 +28,41 @@ Section refinement.
 
   Lemma r_weaken_pre pre pre' post w :
     pre ⇛ pre' ->
-    <{ w : [pre, post] ⊑ w : [pre', post] }>.
+    <{ w : [pre, post] }> ⊑ <{ w : [pre', post] }>.
   Proof.
     intros Hent A Hinit. simpl. f_simpl. assumption.
   Qed.
 
-  Lemma r_assignment : forall pre post (x : ni_variable) t,
-      <! `ni_var_i x` = x ∧ pre !> ⇛ post[x \ t] ->
-      <{ x : [pre, post] ⊑ x := t }>.
+  Lemma r_assignment : forall pre post (x : final_variable) (t : final_term),
+      <! ⌜₀x = x⌝ ∧ pre !> ⇛ post[x \ t] ->
+      <{ x : [pre, post] }> ⊑ <{ x := t }>.
   Proof with auto.
     intros pre post x t H A Hfree. simpl.
-    assert ((ni_formula_formula pre) ≡ pre [x ₀ \ x]).
-    { rewrite fequiv_subst_non_free... pose proof (ni_formula_no_initials pre).
-      destruct (decide (x ₀ ∈ formula_fvars pre))... apply H0 in e. simpl in e. discriminate. }
+    assert (<! %pre !> ≡ pre [₀ x \ x]).
+    { rewrite fequiv_subst_non_free... pose proof (final_formula_final pre).
+      destruct (decide (₀x ∈ formula_fvars pre))... apply H0 in e. simpl in e. discriminate. }
     rewrite H0. clear H0.
     rewrite <- simpl_subst_and.
     rewrite <- (f_forall_one_point).
-    2:{ simpl. rewrite not_elem_of_singleton. apply ni_var_i_ne_ni_var. }
+    2:{ simpl. rewrite not_elem_of_singleton. apply initial_var_of_ne. }
     assert
-      (<! `ni_var_i x` = x => (pre ∧ (∀ x ● post => A)) !> ⇛
-                                <! `ni_var_i x` = x => (post [x \ t] ∧ (∀ x ● post => A)) !>).
+      (<! ⌜₀x = x⌝ ⇒ (pre ∧ (∀ x, post ⇒ A)) !> ⇛
+                                <! ⌜₀x = x⌝ ⇒ (post [x \ t] ∧ (∀ x, post ⇒ A)) !>).
     { intros σ ?. rewrite simpl_feval_fimpl in H0. rewrite simpl_feval_fimpl. intros.
       simp feval in *. apply H0 in H1 as H2. destruct H2 as []. split... apply H.
       simp feval. split... }
     rewrite H0. clear H0. rewrite (f_forall_elim t x). rewrite simpl_subst_impl.
     f_simpl. rewrite f_forall_one_point.
-    2:{ simpl. rewrite not_elem_of_singleton. apply ni_var_i_ne_ni_var. }
+    2:{ simpl. rewrite not_elem_of_singleton. apply initial_var_of_ne. }
     rewrite fequiv_subst_non_free.
-    2:{ destruct (decide (x ₀ ∈ formula_fvars <! A [x \ t] !>))... exfalso.
+    2:{ destruct (decide (₀x ∈ formula_fvars <! A [x \ t] !>))... exfalso.
         apply fvars_subst_superset in e. apply elem_of_union in e. destruct e.
         - apply Hfree in H0. simpl in H0. discriminate.
-        - admit. }
+        - pose proof (final_term_final t). apply H1 in H0. simpl in H0. discriminate. }
     reflexivity.
-  Admitted.
+  Qed.
+
+  Lemma r_alternation
 
   Lemma r_iteration w (I : formula) (v : variable) gcs :
     w : [inv, inv ∧ ¬ (gcomc_any_guard gcs)] ⊑ `PDo gcs`
