src/SeqNotation.v
@@ -1,0 +1,55 @@
+From Stdlib Require Import Lists.List. Import ListNotations.
+From MRC Require Import Prelude.
+
+Declare Custom Entry bracketed_seq_notation.
+Declare Custom Entry seq_notation.
+Declare Custom Entry seq_elem.
+
+Notation "⟨ xs ⟩" := (xs) (in custom bracketed_seq_notation, only parsing,
+                           xs custom seq_elem)
+    : refiney_scope.
+Notation "xs" := (xs) (in custom bracketed_seq_notation at level 0,
+                       only printing,
+                       xs custom seq_elem)
+    : refiney_scope.
+Notation "∅" := ([]) (in custom bracketed_seq_notation at level 0)
+    : refiney_scope.
+Notation "* xs" := xs (in custom bracketed_seq_notation at level 0,
+                         xs constr at level 0,
+                         only parsing)
+    : refiney_scope.
+Notation "*$( xs )" := xs (in custom bracketed_seq_notation at level 0,
+                             xs constr at level 200,
+                             only parsing)
+    : refiney_scope.
+
+
+
+Notation "xs" := (xs) (in custom seq_notation at level 0,
+                       xs custom seq_elem)
+    : refiney_scope.
+Notation "∅" := ([]) (in custom seq_notation at level 0)
+    : refiney_scope.
+
+Notation "x" := ([x]) (in custom seq_elem at level 0, x constr at level 0)
+    : refiney_scope.
+Notation "$( x )" := ([x]) (in custom seq_elem at level 5,
+                           only parsing,
+                             x constr at level 200)
+    : refiney_scope.
+Notation "* x" := x (in custom seq_elem at level 0, x constr at level 0)
+    : refiney_scope.
+Notation "*$( x )" := x (in custom seq_elem at level 5, x constr at level 200)
+    : refiney_scope.
+Notation "x , .. , y" := (app x .. (app y nil) ..)
+                           (in custom seq_elem at level 10,
+                               x custom seq_elem at next level,
+                               y custom seq_elem at next level) : refiney_scope.
+
+(* Open Scope refiney_scope. *)
+(* Notation "'seq' s" := s (at level 10, s custom seq_notation). *)
+
+(* Definition l := [3; 4]. *)
+(* Definition ss : list nat := seq *l. *)
+
+(* Print ss. *)
