src/Prelude.v
@@ -1,2 +1,5 @@
 #[export] Set Default Proof Using "Type".
 #[export] Set Default Goal Selector "!".
+
+Declare Scope refiney_scope.
+Delimit Scope refiney_scope with refiney.
